refactored file structure such that all definitions are three files

src/evaluation.lean
@@ -1,96 +1,6 @@
-/-
-import .syntax .notations
+-- lemmas about evaluation
 
-def unop.apply: unop → value → option value
-| unop.not value.true                    := value.false
-| unop.not value.false                   := value.true
-| unop.isInt (value.num _)               := value.true
-| unop.isInt _                           := value.false
-| unop.isBool value.true                 := value.true
-| unop.isBool value.false                := value.true
-| unop.isBool _                          := value.false
-| unop.isFunc (value.func _ _ _ _ _ _ _) := value.true
-| unop.isFunc _                          := value.false
-| _ _                                    := none
-
-def binop.apply: binop → value → value → option value
-| binop.plus (value.num n₁) (value.num n₂)  := value.num (n₁ + n₂)
-| binop.minus (value.num n₁) (value.num n₂) := value.num (n₁ - n₂)
-| binop.times (value.num n₁) (value.num n₂) := value.num (n₁ * n₂)
-| binop.div (value.num n₁) (value.num n₂)   := value.num (n₁ / n₂)
-| binop.and value.true value.true           := value.true
-| binop.and value.true value.false          := value.false
-| binop.and value.false value.true          := value.false
-| binop.and value.false value.false         := value.false
-| binop.or value.true value.true            := value.true
-| binop.or value.true value.false           := value.true
-| binop.or value.false value.true           := value.true
-| binop.or value.false value.false          := value.false
-| binop.eq v₁ v₂                            := if v₁ = v₂ then value.true else value.false
-| binop.lt (value.num n₁) (value.num n₂)    := if n₁ < n₂ then value.true else value.false
-| _ _ _                                     := none
-
-
-inductive step : stack → stack → Prop
-notation s₁ `⟶` s₂:100 := step s₁ s₂
-
-| ctx {s s': stack} {R: spec} {H: history} {σ: env} {y f x: var} {e: exp}:
-    (s ⟶ s') →
-    (s · [R, H, σ, letapp y = f[x] in e] ⟶ (s' · [R, H, σ, letapp y = f[x] in e]))
-
-| tru {R: spec} {H: history} {σ: env} {x: var} {e: exp}:
-    (R, H, σ, lett x = true in e) ⟶ (R, H, σ[x↦value.true], e)
-
-| fals {R: spec} {H: history} {σ: env} {x: var} {e: exp}:
-    (R, H, σ, letf x = false in e) ⟶ (R, H, σ[x↦value.false], e)
-
-| num {R: spec} {H: history} {σ: env} {x: var} {e: exp} {n: ℤ}:
-    (R, H, σ, letn x = n in e) ⟶ (R, H, σ[x↦value.num n], e)
-
-| closure {H: history} {σ: env} {R' R S: spec} {f x: var} {e₁ e₂: exp}:
-    (R', H, σ, letf f[x] req R ens S {e₁} in e₂) ⟶ 
-    (R', H, σ[f↦value.func f x R S e₁ H σ], e₂)
-
-| unop {R: spec} {H: history} {op: unop} {σ: env} {x y: var} {e: exp} {v₁ v: value}:
-    (σ x = v₁) →
-    (unop.apply op v₁ = v) →
-    ((R, H, σ, letop y = op [x] in e) ⟶ (R, H, σ[y↦v], e))
-
-| binop {R: spec} {H: history} {op: binop} {σ: env} {x y z: var} {e: exp} {v₁ v₂ v: value}:
-    (σ x = v₁) →
-    (σ y = v₂) →
-    (binop.apply op v₁ v₂ = v) →
-    ((R, H, σ, letop2 z = op [x, y] in e) ⟶ (R, H, σ[z↦v], e))
-
-| app {H H': history} {σ σ': env} {R' R S: spec} {f g x y z: var} {e e': exp} {v: value}:
-    (σ f = value.func g z R S e H' σ') →
-    (σ x = v) →
-    ((R', H, σ, letapp y = f[x] in e') ⟶
-    ((R, H', σ'[g↦value.func g z R S e H' σ'][z↦v], e) · [R', H, σ, letapp y = f[x] in e']))
-
-| return {H₁ H₂ H₃: history} {σ₁ σ₂ σ₃: env} {f g gx x y z: var} {R₁ R₂ R S: spec} {e e': exp} {v vₓ: value}:
-    (σ₁ z = v) →
-    (σ₂ f = value.func g gx R S e H₃ σ₃) →
-    (σ₂ x = vₓ) →
-    ((R₁, H₁, σ₁, exp.return z) · [R₂, H₂, σ₂, letapp y = f[x] in e'] ⟶
-    (R₂, H₂ · call g gx R S e H₃ σ₃ vₓ, σ₂[y↦v], e'))
-
-| ite_true {R: spec} {H: history} {σ: env} {e₁ e₂: exp} {x: var}:
-    (σ x = value.true) →
-    ((R, H, σ, exp.ite x e₁ e₂) ⟶ (R, H, σ, e₁))
-
-| ite_false {R: spec} {H: history} {σ: env} {e₁ e₂: exp} {x: var}:
-    (σ x = value.false) →
-    ((R, H, σ, exp.ite x e₁ e₂) ⟶ (R, H, σ, e₂))
-
-notation s₁ `⟶` s₂:100 := step s₁ s₂
-
-inductive trans_step : stack → stack → Prop
-notation s `⟶*` s':100 := trans_step s s'
-| rfl {s: stack}          : s ⟶* s
-| trans {s s' s'': stack} : (s ⟶* s') → (s' ⟶ s'') → (s ⟶* s'')
-
-notation s `⟶*` s':100 := trans_step s s'
+import .definitions2
 
 -- lemmas
 
@@ -99,12 +9,12 @@ lemma binop.eq_of_equal_values {v: value}: binop.apply binop.eq v v = value.true
   show binop.apply binop.eq v v = value.true, by simp[this]
 
 lemma unop.isFunc.inv {v: value}: unop.apply unop.isFunc v = value.true → 
-      ∃ (f x: var) (R S: spec) (e: exp) (H: history) (σ: env), v = value.func f x R S e H σ :=
+      ∃ (f x: var) (R S: spec) (e: exp) (σ: env), v = value.func f x R S e σ :=
   assume isFunc_is_true: unop.apply unop.isFunc v = value.true,
   begin
-    cases v with n f x R S e H σ,
+    cases v with n f x R S e σ,
 
-    show ∃ (f x: var) (R S: spec) (e: exp) (H: history) (σ: env), value.true = value.func f x R S e H σ, from (
+    show ∃ (f x: var) (R S: spec) (e: exp) (σ: env), value.true = value.func f x R S e σ, from (
       have h1: (unop.apply unop.isFunc value.true = value.true), from isFunc_is_true,
       have h2: (unop.apply unop.isFunc value.true = value.false), by unfold unop.apply,
       have some value.true = some value.false, from eq.trans h1.symm h2,
@@ -112,7 +22,7 @@ lemma unop.isFunc.inv {v: value}: unop.apply unop.isFunc v = value.true →
       false.elim (value._mut_.no_confusion this)
     ),
 
-    show ∃ (f x: var) (R S: spec) (e: exp) (H: history) (σ: env), value.false = value.func f x R S e H σ, from (
+    show ∃ (f x: var) (R S: spec) (e: exp) (σ: env), value.false = value.func f x R S e σ, from (
       have h1: (unop.apply unop.isFunc value.false = value.true), from isFunc_is_true,
       have h2: (unop.apply unop.isFunc value.false = value.false), by unfold unop.apply,
       have some value.true = some value.false, from eq.trans h1.symm h2,
@@ -120,7 +30,7 @@ lemma unop.isFunc.inv {v: value}: unop.apply unop.isFunc v = value.true →
       false.elim (value._mut_.no_confusion this)
     ),
 
-    show ∃ (f x: var) (R S: spec) (e: exp) (H: history) (σ: env), value.num n = value.func f x R S e H σ, from (
+    show ∃ (f x: var) (R S: spec) (e: exp) (σ: env), value.num n = value.func f x R S e σ, from (
       have h1: (unop.apply unop.isFunc (value.num n) = value.true), from isFunc_is_true,
       have h2: (unop.apply unop.isFunc (value.num n) = value.false), by unfold unop.apply,
       have some value.true = some value.false, from eq.trans h1.symm h2,
@@ -128,17 +38,17 @@ lemma unop.isFunc.inv {v: value}: unop.apply unop.isFunc v = value.true →
       false.elim (value._mut_.no_confusion this)
     ),
 
-    show ∃ (f_1 x_1: var) (R_1 S_1: spec) (e_1: exp) (H_1: history) (σ_1: env),
-        value.func f x R S e H σ = value.func f_1 x_1 R_1 S_1 e_1 H_1 σ_1, from (
+    show ∃ (f_1 x_1: var) (R_1 S_1: spec) (e_1: exp) (σ_1: env),
+        value.func f x R S e σ = value.func f_1 x_1 R_1 S_1 e_1 σ_1, from (
       exists.intro f (exists.intro x (exists.intro R (exists.intro S
-                     (exists.intro e (exists.intro H (exists.intro σ rfl))))))
+                     (exists.intro e (exists.intro σ rfl)))))
     )
   end
 
 lemma unop.isBool.inv {v: value}: unop.apply unop.isBool v = value.true → (v = value.true) ∨ (v = value.false) :=
   assume isBool_is_true: unop.apply unop.isBool v = value.true,
   begin
-    cases v with n f x R S e H σ,
+    cases v with n f x R S e σ,
 
     show ((value.true = value.true) ∨ (value.true = value.false)), from (
       or.inl rfl
@@ -156,9 +66,9 @@ lemma unop.isBool.inv {v: value}: unop.apply unop.isBool v = value.true → (v =
       false.elim (value._mut_.no_confusion this)
     ),
 
-    show (value.func f x R S e H σ = value.true ∨ (value.func f x R S e H σ = value.false)), from (
-      have h1: unop.apply unop.isBool (value.func f x R S e H σ) = ↑value.true, from isBool_is_true,
-      have h2: (unop.apply unop.isBool (value.func f x R S e H σ) = value.false), by unfold unop.apply,
+    show (value.func f x R S e σ = value.true ∨ (value.func f x R S e σ = value.false)), from (
+      have h1: unop.apply unop.isBool (value.func f x R S e σ) = ↑value.true, from isBool_is_true,
+      have h2: (unop.apply unop.isBool (value.func f x R S e σ) = value.false), by unfold unop.apply,
       have some value.true = some value.false, from eq.trans h1.symm h2,
       have value.true = value.false, from option.some.inj this,
       false.elim (value._mut_.no_confusion this)
@@ -286,7 +196,7 @@ lemma unop_result_not_function {vx vy: value} {op: unop}:
   end
 
 lemma binop_result_not_function {vx vy vz: value} {op: binop}:
-      (binop.apply op vx vy = some vz) → (vz = value.true) ∨ (vz = value.false) ∨ (∃n, vz = value.num n) :=
+      (binop.apply op vx vy = some vz) → ((vz = value.true) ∨ (vz = value.false) ∨ (∃n, vz = value.num n)) :=
   begin
     assume h1,
     cases op,
@@ -554,5 +464,3 @@ lemma binop_result_not_function {vx vy vz: value} {op: binop}:
       unfold binop.apply at h1,
       contradiction    }
   end
-
--/
