src/definitions2.lean
@@ -1,0 +1,656 @@
+-- second part of definitions
+
+import .definitions1 .qiaux
+
+--  ################################
+--  ### QUANTIFIER INSTANTIATION ###
+--  ################################
+
+-- first part is in definitions1.lean
+-- the following definitions need some additional lemmas from qiaux.lean to prove termination
+
+
+-- lift_all(P) performs repeated lifting of quantifiers in positive
+-- positions until there is no more quantifier to be lifted
+def prop.lift_all: prop → prop
+| P :=
+  let r := P.lift_p P.fresh_var in
+  let z := r in
+  have h: z = r, from rfl,
+  @option.cases_on prop (λr, (z = r) → prop) r (
+    assume : z = none,
+    P
+  ) (
+    assume P': prop,
+    assume : z = (some P'),
+    have r_id: r = (some P'), from eq.trans h this,
+    have P'.num_quantifiers < P.num_quantifiers,
+    from (lifted_prop_smaller P').left r_id,
+    prop.lift_all P'
+  ) rfl
+
+using_well_founded {
+  rel_tac := λ _ _, `[exact ⟨_, measure_wf $ λ s, s.num_quantifiers ⟩],
+  dec_tac := tactic.assumption
+}
+
+-- erase_p(P) / erase_n(P) replaces all triggers and quantifiers
+-- in either positive or negative position with 'true'
+mutual def prop.erased_p, prop.erased_n
+
+with prop.erased_p: prop → vc
+| (prop.term t)        := vc.term t
+| (prop.not P)         := have P.sizeof < P.not.sizeof, from sizeof_prop_not,
+                          vc.not P.erased_n
+| (prop.and P₁ P₂)     := have P₁.sizeof < (P₁ ⋀ P₂).sizeof, from sizeof_prop_and₁,
+                          have P₂.sizeof < (P₁ ⋀ P₂).sizeof, from sizeof_prop_and₂,
+                          P₁.erased_p ⋀ P₂.erased_p
+| (prop.or P₁ P₂)      := have P₁.sizeof < (P₁ ⋁ P₂).sizeof, from sizeof_prop_or₁,
+                          have P₂.sizeof < (P₁ ⋁ P₂).sizeof, from sizeof_prop_or₂,
+                          P₁.erased_p ⋁ P₂.erased_p
+| (prop.pre t₁ t₂)     := vc.pre t₁ t₂
+| (prop.pre₁ op t)     := vc.pre₁ op t
+| (prop.pre₂ op t₁ t₂) := vc.pre₂ op t₁ t₂
+| (prop.post t₁ t₂)    := vc.post t₁ t₂
+| (prop.call _)        := vc.term value.true
+| (prop.forallc x P)   := vc.term value.true
+| (prop.exis x P)      := have P.sizeof < (prop.exis x P).sizeof, from sizeof_prop_exis,
+                          vc.not (vc.univ x (vc.not P.erased_p))
+
+with prop.erased_n: prop → vc
+| (prop.term t)        := vc.term t
+| (prop.not P)         := have P.sizeof < P.not.sizeof, from sizeof_prop_not,
+                          vc.not P.erased_p
+| (prop.and P₁ P₂)     := have P₁.sizeof < (P₁ ⋀ P₂).sizeof, from sizeof_prop_and₁,
+                          have P₂.sizeof < (P₁ ⋀ P₂).sizeof, from sizeof_prop_and₂,
+                          P₁.erased_n ⋀ P₂.erased_n
+| (prop.or P₁ P₂)      := have P₁.sizeof < (P₁ ⋁ P₂).sizeof, from sizeof_prop_or₁,
+                          have P₂.sizeof < (P₁ ⋁ P₂).sizeof, from sizeof_prop_or₂,
+                          P₁.erased_n ⋁ P₂.erased_n
+| (prop.pre t₁ t₂)     := vc.pre t₁ t₂
+| (prop.pre₁ op t)     := vc.pre₁ op t
+| (prop.pre₂ op t₁ t₂) := vc.pre₂ op t₁ t₂
+| (prop.post t₁ t₂)    := vc.post t₁ t₂
+| (prop.call _)        := vc.term value.true
+| (prop.forallc x P)   := have P.sizeof < (prop.forallc x P).sizeof, from sizeof_prop_forall,
+                          vc.univ x P.erased_n
+| (prop.exis x P)      := have P.sizeof < (prop.exis x P).sizeof, from sizeof_prop_exis,
+                          vc.not (vc.univ x (vc.not P.erased_n))
+
+using_well_founded {
+  rel_tac := λ _ _, `[exact erased_measure],
+  dec_tac := tactic.assumption
+}
+
+-- given a call trigger t, inst_with_p(P, t) / inst_with_n(P, t) instantiates all quantifiers in
+-- either positive or negative positions by adding a conjunction where the quantified
+-- variable is replaced by the term in the given trigger
+mutual def prop.instantiate_with_p, prop.instantiate_with_n
+
+with prop.instantiate_with_p: prop → calltrigger → prop
+| (prop.term t) _        := prop.term t
+| (prop.not P) t         := have P.sizeof < P.not.sizeof, from sizeof_prop_not,
+                            prop.not (P.instantiate_with_n t)
+| (prop.and P₁ P₂) t     := have P₁.sizeof < (P₁ ⋀ P₂).sizeof, from sizeof_prop_and₁,
+                            have P₂.sizeof < (P₁ ⋀ P₂).sizeof, from sizeof_prop_and₂,
+                            P₁.instantiate_with_p t ⋀ P₂.instantiate_with_p t
+| (prop.or P₁ P₂) t      := have P₁.sizeof < (P₁ ⋁ P₂).sizeof, from sizeof_prop_or₁,
+                            have P₂.sizeof < (P₁ ⋁ P₂).sizeof, from sizeof_prop_or₂,
+                            P₁.instantiate_with_p t ⋁ P₂.instantiate_with_p t
+| (prop.pre t₁ t₂) _     := prop.pre t₁ t₂
+| (prop.pre₁ op t) _     := prop.pre₁ op t
+| (prop.pre₂ op t₁ t₂) _ := prop.pre₂ op t₁ t₂
+| (prop.post t₁ t₂) _    := prop.post t₁ t₂
+| (prop.call t) _        := prop.call t
+| (prop.forallc x P) t   := prop.forallc x P ⋀ P.substt x t.x -- instantiate
+| (prop.exis x P) t      := prop.exis x P
+
+with prop.instantiate_with_n: prop → calltrigger → prop
+| (prop.term t) _        := prop.term t
+| (prop.not P) t         := have P.sizeof < P.not.sizeof, from sizeof_prop_not,
+                            prop.not (P.instantiate_with_p t)
+| (prop.and P₁ P₂) t     := have P₁.sizeof < (P₁ ⋀ P₂).sizeof, from sizeof_prop_and₁,
+                            have P₂.sizeof < (P₁ ⋀ P₂).sizeof, from sizeof_prop_and₂,
+                            P₁.instantiate_with_n t ⋀ P₂.instantiate_with_n t
+| (prop.or P₁ P₂) t      := have P₁.sizeof < (P₁ ⋁ P₂).sizeof, from sizeof_prop_or₁,
+                            have P₂.sizeof < (P₁ ⋁ P₂).sizeof, from sizeof_prop_or₂,
+                            P₁.instantiate_with_n t ⋁ P₂.instantiate_with_n t
+| (prop.pre t₁ t₂) _     := prop.pre t₁ t₂
+| (prop.pre₁ op t) _     := prop.pre₁ op t
+| (prop.pre₂ op t₁ t₂) _ := prop.pre₂ op t₁ t₂
+| (prop.post t₁ t₂) _    := prop.post t₁ t₂
+| (prop.call t) _        := prop.call t
+| (prop.forallc x P) t   := prop.forallc x P
+| (prop.exis x P) t      := prop.exis x P
+
+using_well_founded {
+  rel_tac := λ _ _, `[exact instantiate_with_measure],
+  dec_tac := tactic.assumption
+}
+
+-- finds all call triggers in either positive or negative positions and returns these as list
+mutual def prop.find_calls_p, prop.find_calls_n
+
+with prop.find_calls_p: prop → list calltrigger
+| (prop.term t)        := []
+| (prop.not P)         := have P.sizeof < P.not.sizeof, from sizeof_prop_not,
+                          P.find_calls_n
+| (prop.and P₁ P₂)     := have P₁.sizeof < (P₁ ⋀ P₂).sizeof, from sizeof_prop_and₁,
+                          have P₂.sizeof < (P₁ ⋀ P₂).sizeof, from sizeof_prop_and₂,
+                          P₁.find_calls_p ++ P₂.find_calls_p
+| (prop.or P₁ P₂)      := have P₁.sizeof < (P₁ ⋁ P₂).sizeof, from sizeof_prop_or₁,
+                          have P₂.sizeof < (P₁ ⋁ P₂).sizeof, from sizeof_prop_or₂,
+                          P₁.find_calls_p ++ P₂.find_calls_p
+| (prop.pre t₁ t₂)     := []
+| (prop.pre₁ op t)     := []
+| (prop.pre₂ op t₁ t₂) := []
+| (prop.post t₁ t₂)    := []
+| (prop.call t)        := [ ⟨ t ⟩ ]
+| (prop.forallc x P)   := []
+| (prop.exis x P)      := []
+
+with prop.find_calls_n: prop → list calltrigger
+| (prop.term t)        := []
+| (prop.not P)         := have P.sizeof < P.not.sizeof, from sizeof_prop_not,
+                          P.find_calls_p
+| (prop.and P₁ P₂)     := have P₁.sizeof < (P₁ ⋀ P₂).sizeof, from sizeof_prop_and₁,
+                          have P₂.sizeof < (P₁ ⋀ P₂).sizeof, from sizeof_prop_and₂,
+                          P₁.find_calls_n ++ P₂.find_calls_n
+| (prop.or P₁ P₂)      := have P₁.sizeof < (P₁ ⋁ P₂).sizeof, from sizeof_prop_or₁,
+                          have P₂.sizeof < (P₁ ⋁ P₂).sizeof, from sizeof_prop_or₂,
+                          P₁.find_calls_n ++ P₂.find_calls_n
+| (prop.pre t₁ t₂)     := []
+| (prop.pre₁ op t)     := []
+| (prop.pre₂ op t₁ t₂) := []
+| (prop.post t₁ t₂)    := []
+| (prop.call t)        := []
+| (prop.forallc x P)   := []
+| (prop.exis x P)      := []
+
+using_well_founded {
+  rel_tac := λ _ _, `[exact find_calls_measure],
+  dec_tac := tactic.assumption
+}
+
+-- performs one full instantiation for each of the triggers in the provided list
+def prop.instantiate_with_all: prop → list calltrigger → prop
+| P list.nil        := P
+| P (list.cons t r) := (P.instantiate_with_n t).instantiate_with_all r
+using_well_founded {
+  rel_tac := λ _ _, `[exact ⟨_, measure_wf $ λ s, s.2.sizeof⟩]
+}
+
+-- performs n rounds of instantiations. each round also involves a repeated lifting.
+-- once all rounds are complete, remaining quantifiers and triggers in negative positions will be erased
+def prop.instantiate_rep: prop → ℕ → vc
+| P 0            := P.lift_all.erased_n
+| P (nat.succ n) := have n < n + 1, from lt_of_add_one,
+                    (P.lift_all.instantiate_with_all (P.lift_all.find_calls_n)).instantiate_rep n
+using_well_founded {
+  rel_tac := λ _ _, `[exact ⟨_, measure_wf $ λ s, s.2⟩]
+}
+
+-- finds the maximum quantifier nesting level of a given proposition
+def prop.max_nesting_level: prop → ℕ
+| (prop.term t)        := 0
+| (prop.not P)         := have P.sizeof < P.not.sizeof, from sizeof_prop_not,
+                          P.max_nesting_level
+| (prop.and P₁ P₂)     := have P₁.sizeof < (P₁ ⋀ P₂).sizeof, from sizeof_prop_and₁,
+                          have P₂.sizeof < (P₁ ⋀ P₂).sizeof, from sizeof_prop_and₂,
+                          max P₁.max_nesting_level P₂.max_nesting_level
+| (prop.or P₁ P₂)      := have P₁.sizeof < (P₁ ⋁ P₂).sizeof, from sizeof_prop_or₁,
+                          have P₂.sizeof < (P₁ ⋁ P₂).sizeof, from sizeof_prop_or₂,
+                          max P₁.max_nesting_level P₂.max_nesting_level
+| (prop.pre t₁ t₂)     := 0
+| (prop.pre₁ op t)     := 0
+| (prop.pre₂ op t₁ t₂) := 0
+| (prop.post t₁ t₂)    := 0
+| (prop.call t)        := 0
+| (prop.forallc x P)   := have P.sizeof < (prop.forallc x P).sizeof, from sizeof_prop_forall,
+                          nat.succ P.max_nesting_level
+| (prop.exis x P)      := 0
+
+using_well_founded {
+  rel_tac := λ _ _, `[exact ⟨_, measure_wf $ λ s, s.sizeof⟩],
+  dec_tac := tactic.assumption
+}
+
+-- the main instantiation algorithm performs n rounds of instantiations
+-- where n is the maximum quantifier nesting level and returns the erased proposition
+def prop.instantiated_n (P: prop): vc := P.instantiate_rep P.max_nesting_level
+
+-- top-level calls and quantifiers in positive and negative positions
+mutual inductive prop.has_call_p, prop.has_call_n
+
+with prop.has_call_p: calltrigger → prop → Prop
+| calltrigger {x: term}                                 : prop.has_call_p ⟨x⟩ (prop.call x)
+| not {P: prop} {c: calltrigger}                        : prop.has_call_n c P  → prop.has_call_p c P.not
+| and₁ {P₁ P₂: prop} {c: calltrigger}                   : prop.has_call_p c P₁ → prop.has_call_p c (P₁ ⋀ P₂)
+| and₂ {P₁ P₂: prop} {c: calltrigger}                   : prop.has_call_p c P₂ → prop.has_call_p c (P₁ ⋀ P₂)
+| or₁ {P₁ P₂: prop} {c: calltrigger}                    : prop.has_call_p c P₁ → prop.has_call_p c (P₁ ⋁ P₂)
+| or₂ {P₁ P₂: prop} {c: calltrigger}                    : prop.has_call_p c P₂ → prop.has_call_p c (P₁ ⋁ P₂)
+
+with prop.has_call_n: calltrigger → prop → Prop
+| not {P: prop} {c: calltrigger}                        : prop.has_call_p c P  → prop.has_call_n c P.not
+| and₁ {P₁ P₂: prop} {c: calltrigger}                   : prop.has_call_n c P₁ → prop.has_call_n c (P₁ ⋀ P₂)
+| and₂ {P₁ P₂: prop} {c: calltrigger}                   : prop.has_call_n c P₂ → prop.has_call_n c (P₁ ⋀ P₂)
+| or₁ {P₁ P₂: prop} {c: calltrigger}                    : prop.has_call_n c P₁ → prop.has_call_n c (P₁ ⋁ P₂)
+| or₂ {P₁ P₂: prop} {c: calltrigger}                    : prop.has_call_n c P₂ → prop.has_call_n c (P₁ ⋁ P₂)
+
+-- sets of calls
+def calls_p (P: prop): set calltrigger := λc, prop.has_call_p c P
+def calls_n (P: prop): set calltrigger := λc, prop.has_call_n c P
+
+mutual inductive prop.has_quantifier_p, prop.has_quantifier_n
+
+with prop.has_quantifier_p: callquantifier → prop → Prop
+| callquantifier {x: var} {P: prop}           : prop.has_quantifier_p ⟨x, P⟩ (prop.forallc x P)
+| not {P: prop} {q: callquantifier}           : prop.has_quantifier_n q P  → prop.has_quantifier_p q P.not
+| and₁ {P₁ P₂: prop} {q: callquantifier}      : prop.has_quantifier_p q P₁ → prop.has_quantifier_p q (P₁ ⋀ P₂)
+| and₂ {P₁ P₂: prop} {q: callquantifier}      : prop.has_quantifier_p q P₂ → prop.has_quantifier_p q (P₁ ⋀ P₂)
+| or₁ {P₁ P₂: prop} {q: callquantifier}       : prop.has_quantifier_p q P₁ → prop.has_quantifier_p q (P₁ ⋁ P₂)
+| or₂ {P₁ P₂: prop} {q: callquantifier}       : prop.has_quantifier_p q P₂ → prop.has_quantifier_p q (P₁ ⋁ P₂)
+
+with prop.has_quantifier_n: callquantifier → prop → Prop
+| not {P: prop} {q: callquantifier}           : prop.has_quantifier_p q P  → prop.has_quantifier_n q P.not
+| and₁ {P₁ P₂: prop} {q: callquantifier}      : prop.has_quantifier_n q P₁ → prop.has_quantifier_n q (P₁ ⋀ P₂)
+| and₂ {P₁ P₂: prop} {q: callquantifier}      : prop.has_quantifier_n q P₂ → prop.has_quantifier_n q (P₁ ⋀ P₂)
+| or₁ {P₁ P₂: prop} {q: callquantifier}       : prop.has_quantifier_n q P₁ → prop.has_quantifier_n q (P₁ ⋁ P₂)
+| or₂ {P₁ P₂: prop} {q: callquantifier}       : prop.has_quantifier_n q P₂ → prop.has_quantifier_n q (P₁ ⋁ P₂)
+-- universal quantifiers below existential quantifiers only occur in positive positions,
+-- so can be skolemized instead of instantiated
+
+-- sets of quantifiers
+def quantifiers_p (P: prop): set callquantifier := λc, has_quantifier_p c P
+def quantifiers_n (P: prop): set callquantifier := λc, has_quantifier_n c P
+
+ -- propositions without call triggers or quantifiers do not participate in instantiations
+def no_instantiations(P: prop): Prop := (calls_p P = ∅) ∧ (calls_n P = ∅) ∧
+                                        (quantifiers_p P = ∅) ∧ (quantifiers_n P = ∅)
+
+-- set of calltriggers after substitution
+def calltrigger.subst (σ: env) (c: calltrigger): calltrigger := ⟨term.subst_env σ c.x⟩
+def calls_p_subst (σ: env) (P: prop): set calltrigger := (calltrigger.subst σ) '' calls_p P
+def calls_n_subst (σ: env) (P: prop): set calltrigger := (calltrigger.subst σ) '' calls_n P
+
+--  #############################
+--  ### OPERATIONAL SEMANTICS ###
+--  #############################
+
+-- semantics of unary operators
+def unop.apply: unop → value → option value
+| unop.not value.true                  := value.false
+| unop.not value.false                 := value.true
+| unop.isInt (value.num _)             := value.true
+| unop.isInt _                         := value.false
+| unop.isBool value.true               := value.true
+| unop.isBool value.false              := value.true
+| unop.isBool _                        := value.false
+| unop.isFunc (value.func _ _ _ _ _ _) := value.true
+| unop.isFunc _                        := value.false
+| _ _                                  := none
+
+-- semantics of binary operators
+def binop.apply: binop → value → value → option value
+| binop.plus (value.num n₁) (value.num n₂)  := value.num (n₁ + n₂)
+| binop.minus (value.num n₁) (value.num n₂) := value.num (n₁ - n₂)
+| binop.times (value.num n₁) (value.num n₂) := value.num (n₁ * n₂)
+| binop.div (value.num n₁) (value.num n₂)   := value.num (n₁ / n₂)
+| binop.and value.true value.true           := value.true
+| binop.and value.true value.false          := value.false
+| binop.and value.false value.true          := value.false
+| binop.and value.false value.false         := value.false
+| binop.or value.true value.true            := value.true
+| binop.or value.true value.false           := value.true
+| binop.or value.false value.true           := value.true
+| binop.or value.false value.false          := value.false
+| binop.eq v₁ v₂                            := if v₁ = v₂ then value.true else value.false
+| binop.lt (value.num n₁) (value.num n₂)    := if n₁ < n₂ then value.true else value.false
+| _ _ _                                     := none
+
+-- small-step stack-based semantics
+inductive step : stack → stack → Prop
+notation s₁ `⟶` s₂:100 := step s₁ s₂
+
+| ctx {s s': stack} {R: spec} {σ: env} {y f x: var} {e: exp}:
+    (s ⟶ s') →
+    (s · [R, σ, letapp y = f[x] in e] ⟶ (s' · [R, σ, letapp y = f[x] in e]))
+
+| tru {R: spec} {σ: env} {x: var} {e: exp}:
+    (R, σ, lett x = true in e) ⟶ (R, σ[x↦value.true], e)
+
+| fals {R: spec} {σ: env} {x: var} {e: exp}:
+    (R, σ, letf x = false in e) ⟶ (R, σ[x↦value.false], e)
+
+| num {R: spec} {σ: env} {x: var} {e: exp} {n: ℤ}:
+    (R, σ, letn x = n in e) ⟶ (R, σ[x↦value.num n], e)
+
+| closure {σ: env} {R' R S: spec} {f x: var} {e₁ e₂: exp}:
+    (R', σ, letf f[x] req R ens S {e₁} in e₂) ⟶ 
+    (R', σ[f↦value.func f x R S e₁ σ], e₂)
+
+| unop {R: spec} {op: unop} {σ: env} {x y: var} {e: exp} {v₁ v: value}:
+    (σ x = v₁) →
+    (unop.apply op v₁ = v) →
+    ((R, σ, letop y = op [x] in e) ⟶ (R, σ[y↦v], e))
+
+| binop {R: spec} {op: binop} {σ: env} {x y z: var} {e: exp} {v₁ v₂ v: value}:
+    (σ x = v₁) →
+    (σ y = v₂) →
+    (binop.apply op v₁ v₂ = v) →
+    ((R, σ, letop2 z = op [x, y] in e) ⟶ (R, σ[z↦v], e))
+
+| app {σ σ': env} {R' R S: spec} {f g x y z: var} {e e': exp} {v: value}:
+    (σ f = value.func g z R S e σ') →
+    (σ x = v) →
+    ((R', σ, letapp y = f[x] in e') ⟶
+    ((R, σ'[g↦value.func g z R S e σ'][z↦v], e) · [R', σ, letapp y = f[x] in e']))
+
+| return {σ₁ σ₂ σ₃: env} {f g gx x y z: var} {R₁ R₂ R S: spec} {e e': exp} {v vₓ: value}:
+    (σ₁ z = v) →
+    (σ₂ f = value.func g gx R S e σ₃) →
+    (σ₂ x = vₓ) →
+    ((R₁, σ₁, exp.return z) · [R₂, σ₂, letapp y = f[x] in e'] ⟶
+    (R₂, σ₂[y↦v], e'))
+
+| ite_true {R: spec} {σ: env} {e₁ e₂: exp} {x: var}:
+    (σ x = value.true) →
+    ((R, σ, exp.ite x e₁ e₂) ⟶ (R, σ, e₁))
+
+| ite_false {R: spec} {σ: env} {e₁ e₂: exp} {x: var}:
+    (σ x = value.false) →
+    ((R, σ, exp.ite x e₁ e₂) ⟶ (R, σ, e₂))
+
+notation s₁ `⟶` s₂:100 := step s₁ s₂
+
+-- transitive closure
+inductive trans_step : stack → stack → Prop
+notation s `⟶*` s':100 := trans_step s s'
+| rfl {s: stack}          : s ⟶* s
+| trans {s s' s'': stack} : (s ⟶* s') → (s' ⟶ s'') → (s ⟶* s'')
+
+notation s `⟶*` s':100 := trans_step s s'
+
+--  #######################################
+--  ### VALIDTY OF LOGICAL PROPOSITIONS ###
+--  #######################################
+
+-- validity is axiomatized instead defined
+-- see axioms below
+
+constant valid : vc → Prop
+notation `⊨` p: 20 := valid p
+notation σ `⊨` p: 20 := valid (vc.subst_env σ p)
+notation `⟪` P `⟫`: 100 := ∀ (σ: env), σ ⊨ (prop.instantiated_n P)
+
+-- simple axioms for logical reasoning
+
+axiom valid.tru:
+  ⊨ value.true
+
+axiom valid.and {P Q: vc}:
+  (⊨ P) ∧ (⊨ Q)
+  ↔
+  ⊨ P ⋀ Q
+
+axiom valid.or.left {P Q: vc}:
+  (⊨ P) → 
+  closed Q →
+  ⊨ P ⋁ Q
+
+axiom valid.or.right {P Q: vc}:
+  closed P →
+  (⊨ Q) → 
+  ⊨ P ⋁ Q
+
+axiom valid.or.elim {P Q: vc}:
+  (⊨ P ⋁ Q)
+  →
+  (⊨ P) ∨ (⊨ Q)
+
+axiom valid.not.term {t: term}:
+  (⊨ term.unop unop.not t)
+  ↔
+  ⊨ vc.not t
+
+-- no contradictions
+axiom valid.contradiction {P: vc}:
+  ¬ (⊨ P ⋀ P.not)
+
+-- law of excluded middle
+axiom valid.em {P: vc}:
+  closed P →
+  (⊨ P ⋁ P.not)
+
+-- a term is valid if it equals true
+axiom valid.eq.true {t: term}:
+  ⊨ t
+  ↔
+  ⊨ value.true ≡ t
+
+axiom valid.univ {x: var} {P: vc}:
+  (∀v, ⊨ vc.subst x v P)
+  ↔
+  ⊨ vc.univ x P
+
+-- unary and binary operators are decidable, so equalities with operators are decidable
+axiom valid.unop {op: unop} {vₓ v: value}:
+  unop.apply op vₓ = some v
+  ↔
+  ⊨ v ≡ term.unop op vₓ
+
+axiom valid.binop {op: binop} {v₁ v₂ v: value}:
+  binop.apply op v₁ v₂ = some v
+  ↔
+  ⊨ v ≡ term.binop op v₁ v₂
+
+-- can write pre₁ and pre₂ to check domain of operators
+
+axiom valid.pre₁ {vₓ: value} {op: unop}:
+  option.is_some (unop.apply op vₓ)
+  ↔
+  ⊨ vc.pre₁ op vₓ
+
+axiom valid.pre₂ {v₁ v₂: value} {op: binop}:
+  option.is_some (binop.apply op v₁ v₂)
+  ↔
+  ⊨ vc.pre₂ op v₁ v₂
+
+-- closedness assumption: only closed VCs can be validated
+
+axiom valid.closed {P: vc}:
+  (⊨ P) → closed P
+
+--  #####################################
+--  ### VERIFICATION RELATION (VCGEN) ###
+--  #####################################
+
+reserve infix `⊢`:10
+
+-- verification of expressions
+
+inductive exp.vcgen : prop → exp → propctx → Prop
+notation P `⊢` e `:` Q : 10 := exp.vcgen P e Q
+
+| tru {P: prop} {x: var} {e: exp} {Q: propctx}:
+    x ∉ FV P →
+    (P ⋀ x ≡ value.true ⊢ e : Q) →
+    (P ⊢ lett x = true in e : propctx.exis x (x ≡ value.true ⋀ Q))
+
+| fals {P: prop} {x: var} {e: exp} {Q: propctx}:
+    x ∉ FV P →
+    (P ⋀ x ≡ value.false ⊢ e : Q) →
+    (P ⊢ letf x = false in e : propctx.exis x (x ≡ value.false ⋀ Q))
+
+| num {P: prop} {x: var} {n: ℕ} {e: exp} {Q: propctx}:
+    x ∉ FV P →
+    (P ⋀ x ≡ value.num n ⊢ e : Q) →
+    (P ⊢ letn x = n in e : propctx.exis x (x ≡ value.num n ⋀ Q))
+
+| func {P: prop} {f x: var} {R S: spec} {e₁ e₂: exp} {Q₁ Q₂: propctx}:
+    f ∉ FV P →
+    x ∉ FV P →
+    f ≠ x →
+    x ∈ FV R.to_prop.to_vc →
+    FV R.to_prop ⊆ FV P ∪ { f, x } →
+    FV S.to_prop ⊆ FV P ∪ { f, x } →
+    (P ⋀ spec.func f x R S ⋀ R ⊢ e₁ : Q₁) →
+    (P ⋀ prop.func f x R (Q₁ (term.app f x) ⋀ S) ⊢ e₂ : Q₂) →
+    ⟪prop.implies (P ⋀ spec.func f x R S ⋀ R ⋀ Q₁ (term.app f x)) S⟫ →
+    (P ⊢ letf f[x] req R ens S {e₁} in e₂ : propctx.exis f (prop.func f x R (Q₁ (term.app f x) ⋀ S) ⋀ Q₂))
+
+| unop {P: prop} {op: unop} {e: exp} {x y: var} {Q: propctx}:
+    x ∈ FV P →
+    y ∉ FV P →
+    (P ⋀ y ≡ term.unop op x ⊢ e : Q) →
+    ⟪ prop.implies P (prop.pre₁ op x) ⟫ →
+    (P ⊢ letop y = op [x] in e : propctx.exis y (y ≡ term.unop op x ⋀ Q))
+
+| binop {P: prop} {op: binop} {e: exp} {x y z: var} {Q: propctx}:
+    x ∈ FV P →
+    y ∈ FV P →
+    z ∉ FV P →
+    (P ⋀ z ≡ term.binop op x y ⊢ e : Q) →
+    ⟪ prop.implies P (prop.pre₂ op x y) ⟫ →
+    (P ⊢ letop2 z = op [x, y] in e : propctx.exis z (z ≡ term.binop op x y ⋀ Q))
+
+| app {P: prop} {e: exp} {y f x: var} {Q: propctx}:
+    f ∈ FV P →
+    x ∈ FV P →
+    y ∉ FV P →
+    (P ⋀ prop.call f x ⋀ prop.post f x ⋀ y ≡ term.app f x ⊢ e : Q) →
+    ⟪ prop.implies (P ⋀ prop.call f x) (term.unop unop.isFunc f ⋀ prop.pre f x) ⟫ →
+    (P ⊢ letapp y = f [x] in e : propctx.exis y (prop.call f x ⋀ prop.post f x ⋀ y ≡ term.app f x ⋀ Q))
+
+| ite {P: prop} {e₁ e₂: exp} {x: var} {Q₁ Q₂: propctx}:
+    x ∈ FV P →
+    (P ⋀ x ⊢ e₁ : Q₁) →
+    (P ⋀ prop.not x ⊢ e₂ : Q₂) →
+    ⟪ prop.implies P (term.unop unop.isBool x) ⟫ →
+    (P ⊢ exp.ite x e₁ e₂ : propctx.implies x Q₁ ⋀ propctx.implies (prop.not x) Q₂)
+
+| return {P: prop} {x: var}:
+    x ∈ FV P →
+    (P ⊢ exp.return x : x ≣ •)
+
+notation P `⊢` e `:` Q : 10 := exp.vcgen P e Q
+
+-- verification of environments/translation into logic
+
+inductive env.vcgen : env → prop → Prop
+notation `⊢` σ `:` Q : 10 := env.vcgen σ Q
+
+| empty:
+    ⊢ env.empty : value.true
+
+| tru {σ: env} {x: var} {Q: prop}:
+    x ∉ σ →
+    (⊢ σ : Q) →
+    (⊢ (σ[x ↦ value.true]) : Q ⋀ x ≡ value.true)
+
+| fls {σ: env} {x: var} {Q: prop}:
+    x ∉ σ →
+    (⊢ σ : Q) →
+    (⊢ (σ[x ↦ value.false]) : Q ⋀ x ≡ value.false)
+
+| num {n: ℤ} {σ: env} {x: var} {Q: prop}:
+    x ∉ σ →
+    (⊢ σ : Q) →
+    (⊢ (σ[x ↦ value.num n]) : Q ⋀ x ≡ value.num n)
+
+| func {σ₁ σ₂: env} {f g x: var} {R S: spec} {e: exp} {Q₁ Q₂: prop} {Q₃: propctx}:
+    f ∉ σ₁ →
+    g ∉ σ₂ →
+    x ∉ σ₂ →
+    g ≠ x →
+    (⊢ σ₁ : Q₁) →
+    (⊢ σ₂ : Q₂) →
+    x ∈ FV R.to_prop.to_vc →
+    FV R.to_prop ⊆ FV Q₂ ∪ { g, x } →
+    FV S.to_prop ⊆ FV Q₂ ∪ { g, x } →
+    (Q₂ ⋀ spec.func g x R S ⋀ R ⊢ e : Q₃) →
+    ⟪prop.implies (Q₂ ⋀ spec.func g x R S ⋀ R ⋀ Q₃ (term.app g x)) S⟫ →
+    (⊢ (σ₁[f ↦ value.func g x R S e σ₂]) :
+      (Q₁
+       ⋀ f ≡ value.func g x R S e σ₂
+       ⋀ prop.subst_env (σ₂[g↦value.func g x R S e σ₂]) (prop.func g x R (Q₃ (term.app g x) ⋀ S))))
+
+notation `⊢` σ `:` Q : 10 := env.vcgen σ Q
+
+-- runtime verification of stacks
+
+inductive stack.vcgen : stack → propctx → Prop
+notation `⊢ₛ` s `:` Q : 10 := stack.vcgen s Q
+
+| top {R: spec} {P: prop} {σ: env} {e: exp} {Q: propctx}:
+    (⊢ σ : P) →
+    FV R.to_prop ⊆ FV P →
+    (σ ⊨ R.to_prop.instantiated_n) →
+    (R ⋀ P ⊢ e : Q) →
+    (⊢ₛ (R, σ, e) : P ⋀ Q)
+
+| cons {P₁ P₂ P₃: prop} {s: stack} {σ₁ σ₂: env}
+       {f fx g x y: var} {R₁ R₂ S₂: spec} {e₁ e₂: exp} {v: value} {Q₁ Q₂ Q₂': propctx}:
+    (⊢ₛ s : Q₂') →
+    y ∉ σ₁ →
+    (⊢ σ₁ : P₁) →
+    (⊢ σ₂ : P₂ ) →
+    (⊢ (σ₂[f↦value.func f fx R₂ S₂ e₂ σ₂][fx↦v]) : P₃) →
+    FV R₁.to_prop ⊆ FV P₁ →
+    (σ₁ ⊨ R₁.to_prop.instantiated_n) →
+    (σ₁ g = value.func f fx R₂ S₂ e₂ σ₂) →
+    (σ₁ x = v) →
+    (R₁ ⋀ P₁ ⋀ prop.call g x ⋀ prop.post g x ⋀ y ≡ term.app g x ⊢ e₁ : Q₁) →
+    (P₂ ⋀ spec.func f fx R₂ S₂ ⋀ R₂ ⊢ e₂ : Q₂) →
+    (∀σ' t, (σ' ⊨ (Q₂' t).instantiated_n) → σ' ⊨ (P₃ ⋀ (Q₂ t)).instantiated_n) →
+    (∀v: value, FV (P₃ ⋀ (Q₂ v)) ⊆ FV (Q₂' v)) →
+    ⟪ prop.implies (R₁ ⋀ P₁ ⋀ prop.call g x) (term.unop unop.isFunc g ⋀ prop.pre g x) ⟫ →
+    ((R₂, σ₂[f↦value.func f fx R₂ S₂ e₂ σ₂][fx↦v], e₂) ⟶* s) →
+    (⊢ₛ (s · [R₁, σ₁, letapp y = g[x] in e₁]) : P₁ ⋀
+          propctx.exis y (prop.call g x ⋀ prop.post g x ⋀ y ≡ term.app g x ⋀ Q₁))
+
+notation `⊢ₛ` s `:` Q : 10 := stack.vcgen s Q
+
+
+--  #################################################################
+--  ### AXIOMS ABOUT FUNCTION EXPRESSIONS, PRE and POSTCONDITIONS ###
+--  #################################################################
+
+
+-- The following equality axiom is non-standard and makes validity undecidable.
+-- It is only used in the preservation proof of e-return and in no other lemmas.
+-- The logic treats `f(x)` uninterpreted, so there is no way to derive it naturally.
+-- However, given a complete evaluation derivation of a function call, we can add the
+-- equality `f(x)=y` as new axiom for closed values f, x, y and the resulting set
+-- of axioms is still sound due to deterministic evaluation.
+axiom valid.app {vₓ v: value} {σ σ': env} {f x y: var} {R R' S: spec} {e: exp}:
+  (R, σ[f↦value.func f x R S e σ][x↦vₓ], e) ⟶* (R', σ', exp.return y) →
+  (σ' y = some v)
+  →
+  ⊨ v ≡ term.app (value.func f x R S e σ) vₓ
+
+-- can write pre and post to extract pre- and postcondition of function values
+
+axiom valid.pre.mp {vₓ: value} {σ: env} {f x: var} {R S: spec} {e: exp}:
+  (σ[f↦value.func f x R S e σ][x↦vₓ] ⊨ R.to_prop.to_vc)
+  →
+  ⊨ vc.pre (value.func f x R S e σ) vₓ
+
+axiom valid.pre.mpr {vₓ: value} {σ: env} {f x: var} {R S: spec} {e: exp}:
+  (⊨ vc.pre (value.func f x R S e σ) vₓ)
+  →
+  (σ[f↦value.func f x R S e σ][x↦vₓ] ⊨ R.to_prop.to_vc)
+
+axiom valid.post.mp {vₓ: value} {σ: env} {Q: prop} {Q₂: propctx} {f x: var} {R S: spec} {e: exp}:
+  (⊢ σ : Q) →
+  (Q ⋀ spec.func f x R S ⋀ R ⊢ e : Q₂) →
+  (σ[f↦value.func f x R S e σ][x↦vₓ] ⊨ (Q₂ (term.app f x) ⋀ S.to_prop).to_vc)
+  →
+  (⊨ vc.post (value.func f x R S e σ) vₓ)
+
+axiom valid.post.mpr {vₓ: value} {σ: env} {Q: prop} {Q₂: propctx} {f x: var} {R S: spec} {e: exp}:
+  (⊢ σ : Q) →
+  (Q ⋀ spec.func f x R S ⋀ R ⊢ e : Q₂) →
+  (⊨ vc.post (value.func f x R S e σ) vₓ)
+  →
+  (σ[f↦value.func f x R S e σ][x↦vₓ] ⊨ (Q₂ (term.app f x) ⋀ S.to_prop).to_vc)
