src/qiaux.lean
@@ -1,0 +1,363 @@
+import .definitions1
+
+def prop.num_quantifiers: prop → ℕ
+| (prop.term t)        := 0
+| (prop.not P)         := P.num_quantifiers
+| (prop.and P₁ P₂)     := P₁.num_quantifiers + P₂.num_quantifiers
+| (prop.or P₁ P₂)      := P₁.num_quantifiers + P₂.num_quantifiers
+| (prop.pre t₁ t₂)     := 0
+| (prop.pre₁ op t)     := 0
+| (prop.pre₂ op t₁ t₂) := 0
+| (prop.post t₁ t₂)    := 0
+| (prop.call t)        := 0
+| (prop.forallc x P)   := 1 + P.num_quantifiers
+| (prop.exis x P)      := 1 + P.num_quantifiers
+
+lemma same_num_quantifiers_after_rename {P: prop} {x y: var}:
+      P.num_quantifiers = (P.rename x y).num_quantifiers :=
+  begin
+    induction P,
+    case prop.term t {
+      unfold prop.rename,
+      change (
+        prop.num_quantifiers (prop.term t) =
+        prop.num_quantifiers (prop.term (term.rename x y t))
+      ),
+      unfold prop.num_quantifiers
+    },
+    case prop.not P₁ ih {
+      unfold prop.rename,
+      unfold prop.num_quantifiers,
+      from ih
+    },
+    case prop.and P₁ P₂ P₁_ih P₂_ih {
+      unfold prop.rename,
+      change (
+        prop.num_quantifiers (prop.and P₁ P₂) =
+        prop.num_quantifiers (prop.and (prop.rename x y P₁) (prop.rename x y P₂))
+      ),
+      unfold prop.num_quantifiers,
+      rw[P₁_ih],
+      rw[P₂_ih]
+    },
+    case prop.or P₁ P₂ P₁_ih P₂_ih {
+      unfold prop.rename,
+      change (
+        prop.num_quantifiers (prop.or P₁ P₂) =
+        prop.num_quantifiers (prop.or (prop.rename x y P₁) (prop.rename x y P₂))
+      ),
+      unfold prop.num_quantifiers,
+      rw[P₁_ih],
+      rw[P₂_ih]
+    },
+    case prop.pre t₁ t₂ {
+      unfold prop.rename,
+      unfold prop.num_quantifiers
+    },
+    case prop.pre₁ op t {
+      unfold prop.rename,
+      unfold prop.num_quantifiers
+    },
+    case prop.pre₂ op t₁ t₂ {
+      unfold prop.rename,
+      unfold prop.num_quantifiers
+    },
+    case prop.call t {
+      unfold prop.rename,
+      unfold prop.num_quantifiers
+    },
+    case prop.post t₁ t₂ {
+      unfold prop.rename,
+      unfold prop.num_quantifiers
+    },
+    case prop.forallc y P₁ P₁_ih {
+      unfold prop.rename,
+      by_cases (x = y) with h,
+      
+      simp[h],
+
+      simp[h],
+      unfold prop.num_quantifiers,
+      apply eq_add_left_of_eq,
+      from P₁_ih
+    },
+    case prop.exis y P' P'_ih {
+      unfold prop.rename,
+      by_cases (x = y) with h,
+      
+      simp[h],
+
+      simp[h],
+      unfold prop.num_quantifiers,
+      apply eq_add_left_of_eq,
+      from P'_ih
+    }
+  end
+
+lemma lifted_prop_smaller {P: prop} {x: var}:
+      ∀P', ((P.lift_p x = some P') → (P'.num_quantifiers < P.num_quantifiers)) ∧
+           ((P.lift_n x = some P') → (P'.num_quantifiers < P.num_quantifiers)) :=
+  begin
+    induction P,
+    case prop.term t {
+      assume P',
+      split,
+
+      assume h1,
+      unfold prop.lift_p at h1,
+      contradiction,
+
+      assume h1,
+      unfold prop.lift_n at h1,
+      contradiction
+    },
+    case prop.not P₁ ih {
+      assume P',
+      split,
+
+      assume h1,
+      unfold prop.lift_p at h1,
+      cases h2: prop.lift_n P₁ x,
+
+      simp[h2] at h1,
+      cases h1,
+
+      have h3, from (ih a).right h2,
+      simp[h2] at h1,
+      cases h1,
+      unfold prop.num_quantifiers,
+      from h3,
+
+      assume h1,
+      unfold prop.lift_n at h1,
+      cases h2: prop.lift_p P₁ x,
+
+      simp[h2] at h1,
+      cases h1,
+
+      have h3, from (ih a).left h2,
+      simp[h2] at h1,
+      cases h1,
+      unfold prop.num_quantifiers,
+      from h3
+    },
+    case prop.and P₁ P₂ P₁_ih P₂_ih {
+      assume P',
+      split,
+
+      assume h1,
+      unfold prop.lift_p at h1,
+      cases h2: prop.lift_p P₁ x,
+
+      simp[h2] at h1,
+      cases h3: prop.lift_p P₂ x,
+      simp[h3] at h1,
+      cases h1,
+
+      simp[h3] at h1,
+      cases h1,
+      have h3, from (P₂_ih a).left h3,
+      unfold prop.num_quantifiers,
+      apply nat.add_lt_add_left,
+      from h3,
+
+      simp[h2] at h1,
+      cases h1,
+      unfold prop.num_quantifiers,
+      apply nat.add_lt_add_right,
+      from (P₁_ih a).left h2,
+
+      assume h1,
+      unfold prop.lift_n at h1,
+      cases h2: prop.lift_n P₁ x,
+
+      simp[h2] at h1,
+      cases h3: prop.lift_n P₂ x,
+      simp[h3] at h1,
+      cases h1,
+
+      simp[h3] at h1,
+      cases h1,
+      have h3, from (P₂_ih a).right h3,
+      unfold prop.num_quantifiers,
+      apply nat.add_lt_add_left,
+      from h3,
+
+      simp[h2] at h1,
+      cases h1,
+      unfold prop.num_quantifiers,
+      apply nat.add_lt_add_right,
+      from (P₁_ih a).right h2
+    },
+    case prop.or P₁ P₂ P₁_ih P₂_ih {
+      assume P',
+      split,
+
+      assume h1,
+      unfold prop.lift_p at h1,
+      cases h2: prop.lift_p P₁ x,
+
+      simp[h2] at h1,
+      cases h3: prop.lift_p P₂ x,
+      simp[h3] at h1,
+      cases h1,
+
+      simp[h3] at h1,
+      cases h1,
+      have h3, from (P₂_ih a).left h3,
+      unfold prop.num_quantifiers,
+      apply nat.add_lt_add_left,
+      from h3,
+
+      simp[h2] at h1,
+      cases h1,
+      unfold prop.num_quantifiers,
+      apply nat.add_lt_add_right,
+      from (P₁_ih a).left h2,
+
+      assume h1,
+      unfold prop.lift_n at h1,
+      cases h2: prop.lift_n P₁ x,
+
+      simp[h2] at h1,
+      cases h3: prop.lift_n P₂ x,
+      simp[h3] at h1,
+      cases h1,
+
+      simp[h3] at h1,
+      cases h1,
+      have h3, from (P₂_ih a).right h3,
+      unfold prop.num_quantifiers,
+      apply nat.add_lt_add_left,
+      from h3,
+
+      simp[h2] at h1,
+      cases h1,
+      unfold prop.num_quantifiers,
+      apply nat.add_lt_add_right,
+      from (P₁_ih a).right h2
+    },
+    case prop.pre t₁ t₂ {
+      assume P',
+      split,
+
+      assume h1,
+      unfold prop.lift_p at h1,
+      contradiction,
+
+      assume h1,
+      unfold prop.lift_n at h1,
+      contradiction
+    },
+    case prop.pre₁ op t {
+      assume P',
+      split,
+
+      assume h1,
+      unfold prop.lift_p at h1,
+      contradiction,
+
+      assume h1,
+      unfold prop.lift_n at h1,
+      contradiction
+    },
+    case prop.pre₂ op t₁ t₂ {
+      assume P',
+      split,
+
+      assume h1,
+      unfold prop.lift_p at h1,
+      contradiction,
+
+      assume h1,
+      unfold prop.lift_n at h1,
+      contradiction
+    },
+    case prop.call t {
+      assume P',
+      split,
+
+      assume h1,
+      unfold prop.lift_p at h1,
+      contradiction,
+
+      assume h1,
+      unfold prop.lift_n at h1,
+      contradiction
+    },
+    case prop.post t₁ t₂ {
+      assume P',
+      split,
+
+      assume h1,
+      unfold prop.lift_p at h1,
+      contradiction,
+
+      assume h1,
+      unfold prop.lift_n at h1,
+      contradiction
+    },
+    case prop.forallc y P₁ P₁_ih {
+      assume P',
+      split,
+
+      assume h1,
+      unfold prop.lift_p at h1,
+      have h2, from option.some.inj h1,
+      simp[h2.symm],
+      unfold prop.num_quantifiers,
+      have h3: (prop.num_quantifiers P₁ = prop.num_quantifiers (prop.rename y x P₁)),
+      from same_num_quantifiers_after_rename,
+      rw[←h3],
+      simp,
+      from lt_of_add_one,
+
+      assume h1,
+      unfold prop.lift_n at h1,
+      contradiction
+    },
+    case prop.exis y P₁ P₁_ih {
+      assume P',
+      split,
+
+      assume h1,
+      unfold prop.lift_p at h1,
+      contradiction,
+
+      assume h1,
+      unfold prop.lift_n at h1,
+      have h2, from option.some.inj h1,
+      simp[h2.symm],
+      unfold prop.num_quantifiers,
+      have h3: (prop.num_quantifiers P₁ = prop.num_quantifiers (prop.rename y x P₁)),
+      from same_num_quantifiers_after_rename,
+      rw[←h3],
+      simp,
+      from lt_of_add_one
+    }
+  end
+
+def erased_measure : has_well_founded
+      (psum prop prop)
+:= ⟨_, measure_wf $ λ s,
+  match s with
+  | psum.inl a := a.sizeof
+  | psum.inr a := a.sizeof
+  end⟩
+
+def instantiate_with_measure : has_well_founded
+      (psum (Σ' (p : prop), calltrigger)
+            (Σ' (p : prop), calltrigger))
+:= ⟨_, measure_wf $ λ s,
+  match s with
+  | psum.inl a := a.1.sizeof
+  | psum.inr a := a.1.sizeof
+  end⟩
+
+def find_calls_measure : has_well_founded
+      (psum prop prop)
+:= ⟨_, measure_wf $ λ s,
+  match s with
+  | psum.inl a := a.sizeof
+  | psum.inr a := a.sizeof
+  end⟩
